ulib/FStar.Monotonic.Heap.fst
@@ -1,10 +1,18 @@
-module FStar.Heap
+module FStar.Monotonic.Heap
 
+open FStar.Preorder
 open FStar.Classical
 
+(*
+ * AR: we now need to keep the preorder also in the heap
+ * the reason is that, if we have two references of type a, say r1 and r2, and both the refs are contained in a heap h
+ * then we would like to enforce that their preorders are the same
+ * otherwise, when updating one, we won't be able to prove that the second one also evolves per its preorder
+ * by keeping preorder in the heap, we will ensure in the defn of contains that preorder also matches
+ *)
 private noeq type heap_rec = {
   next_addr: nat;
-  memory   : nat -> Tot (option (a:Type0 & a))
+  memory   : nat -> Tot (option (a:Type0 & rel:(preorder a) & a))
 }
 
 let heap = h:heap_rec{(forall (n:nat). n >= h.next_addr ==> None? (h.memory n))}
@@ -14,41 +22,43 @@ let emp = {
   memory    = (fun (r:nat) -> None)
 }
 
-private type ref' (a:Type0) :Type0 = {
+private type ref' (a:Type0) (rel:preorder a) :Type0 = {
   addr: nat;
   init: a;
   mm:   bool;  //manually managed flag
 }
 
-let ref a = ref' a
+let ref a rel = ref' a rel
 
-let addr_of #a r = r.addr
+let addr_of #a #rel r = r.addr
 
-let is_mm #a r = r.mm
+let is_mm #a #rel r = r.mm
 
-let compare_addrs #a #b r1 r2 = r1.addr = r2.addr
+let compare_addrs #a #b #rel1 #rel2 r1 r2 = r1.addr = r2.addr
 
-let contains #a h r =
+let contains #a #rel h r =
   let _ = () in
-  Some? (h.memory r.addr) /\ dfst (Some?.v (h.memory r.addr)) == a
+  Some? (h.memory r.addr) /\
+  (let (| a1, rel1, _ |) = Some?.v (h.memory r.addr) in
+   a == a1 /\ rel === rel1)  //using `===` here, since otherwise typechecker fails with a and a1 being different types, why?
 
-let unused_in #a r h = None? (h.memory r.addr)
+let unused_in #a #rel r h = None? (h.memory r.addr)
 
-let sel_tot #a h r =
-  let Some (| _, x |) = h.memory r.addr in
+let sel_tot #a #rel h r =
+  let Some (| _, _, x |) = h.memory r.addr in
   x
 
-let sel #a h r =
+let sel #a #rel h r =
   if FStar.StrongExcludedMiddle.strong_excluded_middle (h `contains` r) then
     sel_tot #a h r
   else r.init
 
-let upd_tot #a h r x =
+let upd_tot #a #rel h r x =
   { h with memory = (fun r' -> if r.addr = r'
-			    then Some (| a, x |)
+			    then Some (| a, rel, x |)
                             else h.memory r') }
 
-let upd #a h r x =
+let upd #a #rel h r x =
   if FStar.StrongExcludedMiddle.strong_excluded_middle (h `contains` r)
   then upd_tot h r x
   else
@@ -56,30 +66,30 @@ let upd #a h r x =
     then
       { next_addr = r.addr + 1;
         memory    = (fun (r':nat) -> if r' = r.addr
-	   		         then Some (| a, x |)
+	   		         then Some (| a, rel, x |)
                                  else h.memory r') }
     else
       { h with memory = (fun r' -> if r' = r.addr
-				then Some (| a, x |)
+				then Some (| a, rel, x |)
                                 else h.memory r') }
 
-let alloc #a h x mm =
+let alloc #a rel h x mm =
   let r = { addr = h.next_addr; init = x; mm = mm } in
-  r, upd #a h r x
+  r, upd #a #rel h r x
 
-let free_mm #a h r =
+let free_mm #a #rel h r =
   { h with memory = (fun r' -> if r' = r.addr then None else h.memory r') }
 
 (*
  * update of a well-typed reference
  *)
 private let lemma_upd_contains_test
-  (#a:Type) (h0:heap) (r:ref a) (x:a)
+  (#a:Type) (#rel:preorder a) (h0:heap) (r:ref a rel) (x:a{valid_upd h0 r x})
   :Lemma (h0 `contains` r ==>
           (let h1 = upd h0 r x in
-           (forall (b:Type) (r':ref b). addr_of r' <> addr_of r ==> sel h0 r' == sel h1 r') /\
-	   (forall (b:Type) (r':ref b). h0 `contains` r' <==> h1 `contains` r')             /\
-	   (forall (b:Type) (r':ref b). r' `unused_in` h0  <==> r' `unused_in` h1)))
+           (forall (b:Type) (rel:preorder b) (r':ref b rel). addr_of r' <> addr_of r ==> sel h0 r' == sel h1 r') /\
+	   (forall (b:Type) (rel:preorder b) (r':ref b rel). h0 `contains` r' <==> h1 `contains` r')             /\
+	   (forall (b:Type) (rel:preorder b) (r':ref b rel). r' `unused_in` h0  <==> r' `unused_in` h1)))
   = ()
 
 (*
@@ -90,74 +100,74 @@ private let lemma_upd_contains_test
  * in h0, r' is well-typed, but in h1 it's not
  *)
 private let lemma_upd_contains_not_necessarily_well_typed_test
-  (#a:Type) (h0:heap) (r:ref a) (x:a)
+  (#a:Type) (#rel:preorder a) (h0:heap) (r:ref a rel) (x:a{valid_upd h0 r x})
   :Lemma ((~ (r `unused_in` h0)) ==>
           (let h1 = upd h0 r x in
 	   h1 `contains` r /\
-           (forall (b:Type) (r':ref b). addr_of r' <> addr_of r ==> sel h0 r' == sel h1 r')           /\
-	   (forall (b:Type) (r':ref b). (r'.addr <> r.addr /\ h0 `contains` r') ==> h1 `contains` r') /\
-	   (forall (b:Type) (r':ref b). r' `unused_in` h0 <==> r' `unused_in` h1)))
+           (forall (b:Type) (#rel:preorder b) (r':ref b rel). addr_of r' <> addr_of r ==> sel h0 r' == sel h1 r')           /\
+	   (forall (b:Type) (#rel:preorder b) (r':ref b rel). (r'.addr <> r.addr /\ h0 `contains` r') ==> h1 `contains` r') /\
+	   (forall (b:Type) (#rel:preorder b) (r':ref b rel). r' `unused_in` h0 <==> r' `unused_in` h1)))
   = ()
 
 (*
  * update of an unused reference
  *)
 private let lemma_upd_unused_test
-  (#a:Type) (h0:heap) (r:ref a) (x:a)
+  (#a:Type) (#rel:preorder a) (h0:heap) (r:ref a rel) (x:a{valid_upd h0 r x})
   :Lemma (r `unused_in` h0 ==>
           (let h1 = upd h0 r x in
 	   h1 `contains` r /\
-           (forall (b:Type) (r':ref b). addr_of r' <> addr_of r ==> sel h0 r' == sel h1 r') /\
-	   (forall (b:Type) (r':ref b). h0 `contains` r' ==> h1 `contains` r')             /\
-	   (forall (b:Type) (r':ref b). ~ (r' `unused_in` h0) ==> ~ (r' `unused_in` h1))))
+           (forall (b:Type) (rel:preorder b) (r':ref b rel). addr_of r' <> addr_of r ==> sel h0 r' == sel h1 r') /\
+	   (forall (b:Type) (rel:preorder b) (r':ref b rel). h0 `contains` r' ==> h1 `contains` r')             /\
+	   (forall (b:Type) (rel:preorder b) (r':ref b rel). ~ (r' `unused_in` h0) ==> ~ (r' `unused_in` h1))))
   = ()
 
 (*
  * alloc and alloc_mm behaves just like upd of an unmapped reference
  *)
-private let lemma_alloc_test (#a:Type) (h0:heap) (x:a) (mm:bool)
-  :Lemma (let (r, h1) = alloc h0 x mm in
+private let lemma_alloc_test (#a:Type) (rel:preorder a) (h0:heap) (x:a) (mm:bool)
+  :Lemma (let (r, h1) = alloc rel h0 x mm in
           r `unused_in` h0 /\
 	  h1 `contains` r  /\
           is_mm r = mm     /\
-          (forall (b:Type) (r':ref b). addr_of r' <> addr_of r ==> sel h0 r' == sel h1 r') /\
-          (forall (b:Type) (r':ref b). h0 `contains` r' ==> h1 `contains` r')             /\
-	  (forall (b:Type) (r':ref b). ~ (r' `unused_in` h0) ==> ~ (r' `unused_in` h1)))
+          (forall (b:Type) (rel:preorder b) (r':ref b rel). addr_of r' <> addr_of r ==> sel h0 r' == sel h1 r') /\
+          (forall (b:Type) (rel:preorder b) (r':ref b rel). h0 `contains` r' ==> h1 `contains` r')             /\
+	  (forall (b:Type) (rel:preorder b) (r':ref b rel). ~ (r' `unused_in` h0) ==> ~ (r' `unused_in` h1)))
   = ()
 
-private let lemma_free_mm_test (#a:Type) (h0:heap) (r:ref a{h0 `contains` r /\ is_mm r})
+private let lemma_free_mm_test (#a:Type) (rel:preorder a) (h0:heap) (r:ref a rel{h0 `contains` r /\ is_mm r})
   :Lemma (let h1 = free_mm h0 r in
           r `unused_in` h1 /\
-	  (forall (b:Type) (r':ref b). addr_of r' <> addr_of r ==>
+	  (forall (b:Type) (rel:preorder b) (r':ref b rel). addr_of r' <> addr_of r ==>
 	                          ((sel h0 r' == sel h1 r'                 /\
 				   (h0 `contains` r' <==> h1 `contains` r') /\
 				   (r' `unused_in` h0 <==> r' `unused_in` h1)))))
   = ()
 
-private let lemma_alloc_fresh_test (#a:Type) (h0:heap) (x:a) (mm:bool)
-  :Lemma (let r, h1 = alloc h0 x mm in
+private let lemma_alloc_fresh_test (#a:Type) (rel:preorder a) (h0:heap) (x:a) (mm:bool)
+  :Lemma (let r, h1 = alloc rel h0 x mm in
           fresh r h0 h1 /\ modifies Set.empty h0 h1)
   = ()
 
-let lemma_contains_implies_used #a h r = ()
-let lemma_distinct_addrs_distinct_types #a #b h r1 r2 = ()
-let lemma_distinct_addrs_unused #a #b h r1 r2 = ()
-let lemma_alloc #a h0 x mm = ()
-let lemma_free_mm_sel #a #b h0 r1 r2 = ()
-let lemma_free_mm_contains #a #b h0 r1 r2 = ()
-let lemma_free_mm_unused #a #b h0 r1 r2 = ()
-let lemma_sel_same_addr #a h r1 r2 = ()
-let lemma_sel_upd1 #a h r1 x r2 = ()
-let lemma_sel_upd2 #a #b h r1 r2 x = ()
+let lemma_contains_implies_used #a #rel h r = ()
+let lemma_distinct_addrs_distinct_types #a #b #rel1 #rel2 h r1 r2 = ()
+let lemma_distinct_addrs_unused #a #b #rel1 #rel2 h r1 r2 = ()
+let lemma_alloc #a rel h0 x mm = ()
+let lemma_free_mm_sel #a #b #rel1 #rel2 h0 r1 r2 = ()
+let lemma_free_mm_contains #a #b #rel1 #rel2 h0 r1 r2 = ()
+let lemma_free_mm_unused #a #b #rel1 #rel2 h0 r1 r2 = ()
+let lemma_sel_same_addr #a #rel h r1 r2 = ()
+let lemma_sel_upd1 #a #rel h r1 x r2 = ()
+let lemma_sel_upd2 #a #b #rel1 #rel2 h r1 r2 x = ()
 let lemma_ref_injectivity = ()
-let lemma_in_dom_emp #a r = ()
-let lemma_upd_contains #a h r x = ()
-let lemma_well_typed_upd_contains #a #b h r1 x r2 = ()
-let lemma_unused_upd_contains #a #b h r1 x r2 = ()
-let lemma_upd_contains_different_addr #a #b h r1 x r2 = ()
-let lemma_upd_unused #a #b h r1 x r2 = ()
-let lemma_contains_upd_modifies #a h r x = ()
-let lemma_unused_upd_modifies #a h r x = ()
+let lemma_in_dom_emp #a #rel r = ()
+let lemma_upd_contains #a #rel h r x = ()
+let lemma_well_typed_upd_contains #a #b #rel1 #rel2 h r1 x r2 = ()
+let lemma_unused_upd_contains #a #b #rel1 #rel2 h r1 x r2 = ()
+let lemma_upd_contains_different_addr #a #b #rel1 #rel2 h r1 x r2 = ()
+let lemma_upd_unused #a #b #rel1 #rel2 h r1 x r2 = ()
+let lemma_contains_upd_modifies #a #rel h r x = ()
+let lemma_unused_upd_modifies #a #rel h r x = ()
 
 let equal h1 h2 =
   let _ = () in
@@ -166,4 +176,4 @@ let equal h1 h2 =
 
 let equal_extensional h1 h2 = ()
 
-let upd_upd_same_ref #a h r x y = assert (equal (upd (upd h r x) r y) (upd h r y))
+let upd_upd_same_ref #a #rel h r x y = assert (equal (upd (upd h r x) r y) (upd h r y))
